\begin{sol}
Conservation of momentum and energy gives us (neglecting powers of $c$):
\begin{align*}
    p_\gamma + p_1 &= p_2 \\
    p_\gamma + \sqrt{m_e^2+p_1^2} &=  \sqrt{m_e^2+p_2^2}
\end{align*}
Squaring and solving will give us:
$$
(p_{2}-p_{1})^{2} - (p_{2}^{2}-p_{1}^{2}) +
2(p_{2}-p_{1})\sqrt{(p_{1}^{2}+m_{e}^{2})} = 0
$$
One obvious solution is $p_2-p_1=0$ but this is only achieved when $p_\gamma=0$ which cannot be possible. Dividing through by this factor, we are left with:
$$
\sqrt{(p_{1}^{2}+m_{e}^{2})} - p_{1} =0
$$
which can only be possible if $m_e = 0$ which it certainly is not.
\end{sol}