\begin{sol}
\begin{enumerate}[label=\textbf{(\alph*)}]
\item First, note that, by the normalization condition, the following is true: $$N^2\int_{-\infty}^{\infty}\psi(x)\;\psi^*(x)\;\mathrm{d}x = N^2\int_{-\infty}^{\infty}\operatorname{exp}\left(-\frac{x^2}{a^2}\right)\;\mathrm{d}x = 1$$
Also, note that by the symmetry of the situation, $\left<x\right>$ must be zero. However, we can also show this through calculation.
\begin{align*}
    \left(\Delta x\right)^2 &= \left<x^2\right> - \left<x\right>^2\\ &= \int_{-\infty}^{\infty}\psi^*(x)\;\hat{x}^2\;\psi(x)\;\mathrm{d}x -\left(\int_{-\infty}^{\infty}\psi^*(x)\;\hat{x}\;\psi(x)\;\mathrm{d}x\right)^2\\ &= N^2\int_{-\infty}^{\infty}x^2\operatorname{exp}\left(-\frac{x^2}{a^2}\right)\;\mathrm{d}x -\left(N^2\int_{-\infty}^{\infty}x\operatorname{exp}\left(-\frac{x^2}{a^2}\right)\mathrm{d}x\right)^2\\ &= \frac{1}{2}a^2N^2\int_{-\infty}^{\infty}\operatorname{exp}\left(-\frac{x^2}{a^2}\right)\;\mathrm{d}x - 0 \\ &= \frac{1}{2}a^2
\end{align*}
Similarly, it can be said that $\left<p\right>$ is zero by the symmetry of the situation (prove this using the integral definition of expectation values if you wish, in a similar manner to how it was proved above).
\begin{align*}
\left(\Delta p\right)^2 &= \left<p^2\right> - \left<p\right>^2 \\ &= \int_{-\infty}^{\infty}\psi^*(x)\;\hat{p}^2\;\psi(x)\;\mathrm{d}x - 0 \\ &= -\hbar^2N^2\int_{-\infty}^{\infty}\operatorname{exp}\left(-\frac{x^2}{2a^2}\right)\frac{\partial^2}{\partial x^2}\left(\operatorname{exp}\left(-\frac{x^2}{2a^2}\right)\right)\;\mathrm{d}x \\ &= -\frac{\hbar^2N^2}{a^4}\int_{-\infty}^{\infty}(x^2-a^2)\;\operatorname{exp}\left(-\frac{x^2}{a^2}\right)\mathrm{d}x \\ &= -\frac{\hbar^2N^2}{2a^2}\int_{-\infty}^{\infty}\operatorname{exp}\left(-\frac{x^2}{a^2}\right)\;\mathrm{d}x + \frac{\hbar^2N^2}{a^2}\int_{-\infty}^{\infty}\operatorname{exp}\left(-\frac{x^2}{a^2}\right)\mathrm{d}x\\ &= -\frac{\hbar^2}{2a^2} + \frac{\hbar^2}{a^2} \\ &= \frac{\hbar^2}{2a^2}
\end{align*}
Then, $$\Delta x\Delta p = \sqrt{\frac{a^2}{2}\frac{\hbar^2}{2a^2}} = \frac{\hbar}{2}$$ which does in fact saturate the Heisenberg uncertainty product.
\item
\begin{align*}
\phi(p) &= \frac{1}{\sqrt{2\pi\hbar}}\int_{-\infty}^{\infty}\psi(x)\;e^{-ipx/\hbar}\;\mathrm{d}x \\ &= \frac{N}{\sqrt{2\pi\hbar}}\int_{-\infty}^{\infty}\operatorname{exp}\left(-\frac{x^2}{2a^2} - \frac{ipx}{\hbar}\right)\mathrm{d}x \\ &= \frac{N}{\sqrt{2\pi\hbar}}\sqrt{2\pi a^2}\operatorname{exp}\left(-\frac{p^2a^2}{2\hbar^2}\right) \\ &= \frac{Na}{\sqrt{\hbar}}\operatorname{exp}\left(-\frac{p^2a^2}{2\hbar^2}\right)
\end{align*}We can verify this is correct by ensuring the normalization condition is met, as required by Parseval's Theorem. $$\int_{-\infty}^{\infty}\phi(p)\phi^*(p)\;\mathrm{d}p = \frac{N^2a^2}{\hbar}\int_{-\infty}^{\infty}\operatorname{exp}\left(-\frac{p^2a^2}{\hbar^2}\right)\mathrm{d}p = N^2a\sqrt{\pi} = 1$$In fact, this is the same normalization condition obtained for the position wavefunction (which can be shown similarly), which lines up with Parseval's theorem and proves our wavefunction is correct. Then, \begin{align*}
\left(\Delta p\right)^2 &= \left<p^2\right> - \left<p\right>^2 \\ &= \left<p^2\right> - 0 \\ &= \int_{-\infty}^{\infty}\phi^*(p)\;\hat{p}^2\;\phi(p)\;\mathrm{d}p\\ &= \frac{N^2a^2}{\hbar}\int_{-\infty}^{\infty}p^2\operatorname{exp}\left(-\frac{p^2a^2}{\hbar^2}\right)\mathrm{d}p \\ &= \frac{\hbar^2}{2a^2}\frac{N^2a^2}{\hbar}\int_{-\infty}^{\infty}\operatorname{exp}\left(-\frac{p^2a^2}{\hbar^2}\right)\mathrm{d}p \\ &= \frac{\hbar^2}{2a^2}
\end{align*}This result lines up with what was calculated using the position wavefunction.
\end{enumerate}
\end{sol}



