\begin{sol}
First, we prove the fact stated in the problem for $z = re^{i\theta}$: $$\frac{\operatorname{Re}(z)}{|z|^2} = \frac{r\cos\theta}{r^2} = \frac{\cos\theta}{r} = \frac{\cos{\left(-\theta\right)}}{r} = \operatorname{Re}\left(\frac{1}{z}\right)$$ Also, note by the normalization condition that: $$\int_{-\infty}^{\infty}|\psi(x)|^2\;\mathrm{d}x = N^2\int_{-\infty}^{\infty}\operatorname{exp}\left(\operatorname{Re}\left(-\frac{x^2}{2\Delta^2}\right)\right)^2\mathrm{d}x = N^2\int_{-\infty}^{\infty}\operatorname{exp}\left(-\frac{x^2\operatorname{Re}\left(\Delta^2\right)}{|\Delta|^4}\right)\mathrm{d}x =1$$
\begin{enumerate}[label=\textbf{(\alph*)}]
\item For both momentum and position calculations, we can again note by symmetry that $\left<x\right>=0$ and $\left<p\right>=0$. Then,
\begin{align*}
\left(\Delta x\right)^2 &= \left<x^2\right> - 0^2\\ &= \int_{-\infty}^{\infty}\psi^*(x)\;\hat{x}^2\;\psi(x)\;\mathrm{d}x \\ &= \int_{-\infty}^{\infty}x^2\;|\psi(x)|^2\;\mathrm{d}x \\ &= N^2\int_{-\infty}^{\infty}x^2\operatorname{exp}\left(\operatorname{Re}\left(-\frac{x^2}{2\Delta^2}\right)\right)^2\mathrm{d}x \\ &= N^2\int_{-\infty}^{\infty}x^2\operatorname{exp}\left(-\frac{x^2\operatorname{Re}\left(\Delta^2\right)}{|\Delta|^4}\right)\mathrm{d}x \\ &= \frac{|\Delta|^4}{2\operatorname{Re}\left(\Delta^2\right)}N^2\int_{-\infty}^{\infty}\operatorname{exp}\left(-\frac{x^2\operatorname{Re}\left(\Delta^2\right)}{|\Delta|^4}\right)\mathrm{d}x \\ &= \frac{|\Delta|^4}{2\operatorname{Re}\left(\Delta^2\right)}
\end{align*}
\begin{align*}
\left(\Delta p\right)^2 &= \left<p^2\right> - 0^2  \\ &= \int_{-\infty}^{\infty}\psi^*(x)\;\hat{p}^2\;\psi(x)\;\mathrm{d}x \\ &= -\hbar^2N^2\int_{-\infty}^{\infty}\operatorname{exp}^*\left(-\frac{x^2}{2\Delta^2}\right)\frac{\partial^2}{\partial x^2}\left(\operatorname{exp}\left(-\frac{x^2}{2\Delta^2}\right)\right) \\ &= -\frac{\hbar^2N^2}{\Delta^4}\int_{-\infty}^{\infty}\left(x^2 -\Delta^2\right)\operatorname{exp}\left(-\frac{x^2\operatorname{Re}\left(\Delta^2\right)}{|\Delta|^4}\right)\mathrm{d}x \\ &= -\frac{\hbar^2N^2|\Delta|^4}{2\Delta^4\operatorname{Re}\left(\Delta^2\right)}\int_{-\infty}^{\infty}\operatorname{exp}\left(-\frac{x^2\operatorname{Re}\left(\Delta^2\right)}{|\Delta|^4}\right)\mathrm{d}x + \frac{\hbar^2N^2}{\Delta^2}\int_{-\infty}^{\infty}\operatorname{exp}\left(-\frac{x^2\operatorname{Re}\left(\Delta^2\right)}{|\Delta|^4}\right)\mathrm{d}x \\ &= -\frac{\hbar^2|\Delta|^4}{2\Delta^4\operatorname{Re}\left(\Delta^2\right)}+ \frac{\hbar^2}{\Delta^2}
\end{align*}
Letting $|\Delta|^4=(\Delta^2)^*\Delta^2$ and $2\Re(\Delta^2)=(\Delta^2)^*+\Delta^2$, we can simplify this expression to
$$(\Delta p)^2 = \frac{\hbar^2}{2\Re(\Delta^2)}$$
\item \begin{align*}
\phi(p) &= \frac{1}{\sqrt{2\pi\hbar}}\int_{-\infty}^{\infty}\psi(x)\;e^{-ipx/\hbar}\;\mathrm{d}x \\ &= \frac{N}{\sqrt{2\pi\hbar}}\int_{-\infty}^{\infty}\operatorname{exp}\left(-\frac{x^2}{2\Delta^2} - \frac{ipx}{\hbar}\right)\mathrm{d}x \\ &= \frac{N}{\sqrt{2\pi\hbar}}\sqrt{2\pi\Delta^2}\operatorname{exp}\left(-\frac{p^2\Delta^2}{2\hbar^2}\right) \\ &= \frac{N\Delta}{\sqrt{\hbar}}\operatorname{exp}\left(-\frac{p^2\Delta^2}{2\hbar^2}\right)
\end{align*}
This result can be shown to be correct using Parseval's Theorem:
\begin{align*}
    1 &= \int_{-\infty}^{\infty} |\Phi(p)|^2 dp \\
    &= \frac{N^2|\Delta|^2}{\hbar}\int_{-\infty}^{\infty} \exp\left(-\frac{p^2\Re(\Delta^2)}{\hbar^2}\right)dp\\
    &= N^2|\Delta|^2\sqrt{\frac{\pi}{\Re(\Delta^2)}}
\end{align*}
This is the same normalization condition that we originally stated where we worked in position space. The uncertainty is thus
\begin{align*}
    (\Delta p)^2 &= \int_{-\infty}^{\infty} p^2|\Phi|^2 dp \\
    &= \frac{N^2|\Delta|^2}{\hbar}\int_{-\infty}^{\infty}p^2\exp\left(\frac{-p^2}{\hbar^2}\Re(\Delta^2)\right) dp \\
    &= \frac{\hbar^2}{2\Re(\Delta^2)}\frac{N^2|\Delta|^2}{\hbar}\int_{-\infty}^{\infty}\exp\left(\frac{-p^2}{\hbar^2}\Re(\Delta^2)\right) dp \\
    &= \frac{\hbar^2}{2\Re(\Delta^2)}
\end{align*}
where we have used our earlier normalization condition.
\item We have:
\begin{align*}
    (\Delta x\Delta p)^2 &= \frac{\hbar^2}{4}\left(\frac{|\Delta|^4}{\Re(\Delta^2)^2}\right) \\
    &= \frac{\hbar^2}{4}\left(\frac{|\Delta|^4}{\Re(|\Delta|^2e^{i2\Phi_\Delta})^2}\right) \\
    &= \frac{\hbar^2}{4}\left(\frac{|\Delta|^4}{(|\Delta|^2\cos(2\phi_\Delta))^2}\right) \\
    \Delta x\Delta p &= \frac{\hbar}{2\cos(2\Phi_\Delta)}
\end{align*}
For $\Phi_\Delta=0$, then $\Delta$ becomes real and it becomes identical to the first problem. For $\Phi_\Delta \to \pi/4$, the product $\Delta x\Delta p \to \infty$. This is because at this limit, $\Delta^2$ becomes purely imaginary. Thus, we get a pure phase with a constant oscillation and no dampening effect, causing there to be infinite momentum and position eigenstates with the same probability, causing their uncertainty to become infinite as well. 
\item In problem three, the given wavefunction was:
$$\Psi = N\exp\left(-\frac{x^2}{4a^2}\right)$$
Therefore, $\Delta^2=2a^2$. The uncertainty at $t=0$ is then:
$$(\Delta p)^2=\frac{\hbar^2}{2a^2}$$
Including the time dependence, the wavefunction becomeS:
$$\Psi(x,t)=N\exp\left(-\frac{mx^2}{2\hbar(\tau+it)}\right)$$
where $\tau=\frac{2ma^2}{\hbar}$. Therefore:
$$
\Delta^2 = \frac{\hbar(\tau+it)}{m}
$$
and
$$
\Re(\Delta^2)=\frac{\hbar\tau}{m} \implies \Delta^2=2a^2
$$
which is equivalent to the time $t=0$ case, showing that the momentum uncertainty is indeed time independent.
\end{enumerate}
\end{sol}