\begin{sol}
\begin{enumerate}[label=\textbf{(\alph*)}]
\item To show that the field satisfies the EM wave equation we first write the EM wave equation as 
\[\vec{\nabla}^2 E = \frac{1}{c^2}\pdv{^{2}\vec{E}}{t^2}.\]
We see that $\vec{\nabla}^2 E$ is given by 
\[\vec{\nabla}^2 E = \left(\pdv{^2}{x^2} + \pdv{^2}{y^2} + \pdv{^2}{z^2}\right)\vec{E}.\]
Since the EM wave only goes in the $\hat{y}$ direction, this means that 
\[\vec{\nabla}^2 E = \pdv{^2 E_y}{x^2}\hat{y} = E f^{\prime \prime} (x - ct)\hat{y}.\]
Also, 
\[\pdv{^2 \vec{E}}{t^2} = c^2 E_0 f^{\prime \prime} (x - ct)\hat{y}.\]
This now clearly satisfies the EM wave equation.

\item We note that 
\[\vec{\nabla}\cdot \vec{E} = \left(\pdv{^2 E_x}{x^2} + \pdv{^2 E_y}{y^2} + \pdv{^2 E_z}{z^2}\right) = 0\]
as long as $E_x = 0$.

\item Note that 
\[\vec{\nabla}\times \vec{E} = -\pdv{\vec{B}}{t} \implies -\pdv{\vec{B}}{t} = 
\begin{vmatrix}
\hat{x} & \hat{y} & \hat{z} \\
\pdv{}{x} & \pdv{}{y} & \pdv{}{z} \\
0 & E_y & 0
\end{vmatrix}.
\]
This tells us that 
\[-\pdv{\vec{B}}{t} = \pdv{E_y}{x} \hat{z}\implies \vec{B} = \boxed{\frac{E_0}{c} f (x - ct) \hat{z}}.\]
\end{enumerate}
\end{sol}