\begin{sol}
\begin{enumerate}[label=\textbf{(\alph*)}]
\item When the crystal is displaced a distance $x$ from the equilibrium position, our equation of motion will be predetermined by 
\[M\ddot{x} = F - k_{\text{eff}} x - Mg.\]
Substituting $F = MA_0 \cos (\omega_d t)$ and $k_{\text{eff}} = 4k$ into our equation gives us our equation of motion to be
\[\boxed{M\ddot{x} = MA_0 \cos (\omega_d t) - 4k (A_0 - x) - Mg}.\]

\item Now, since the homogeneous solution dies out eventually there should be a very small drag force, we add the drag force factor of $-\gamma \dot{x}$ to our equation. We now have our equation of motion to be 
\[M\ddot{x} = MA_0 \cos (\omega_d t) - 4kx - Mg - \gamma \dot{x}\]
and rearranging gives us 
\[M\ddot{x} + \gamma \dot{x} + 4kx = MA_0 \cos (\omega_d t).\]
Note that this equation is very similar to the one discussed and solved in lecture 3:
\[\ddot\theta + \Gamma \dot\theta + \omega_0^2 \theta = f_0 \cos (\omega_d t).\]
Dividing by $M$ on both sides of our obtained equation gives us the form 
\[\ddot{x} + \frac{\gamma}{M}\dot{x} + \frac{4k}{M}x = A_0 \cos (\omega_d t)\]
which now tells us that 
\begin{align*}
    \Gamma &= \frac{\gamma}{M},\\
    \omega_0^2 &= \frac{4k}{M}\implies \omega_0 = \sqrt{\frac{4k}{M}}\\
    f_0 &= A_0.
\end{align*}
As solved in the lecture, the amplitude of oscillations of this equation is given by 
\[A = \frac{f_0}{\sqrt{(\omega_0^2 - \omega_d^2)^2 + \omega_d^2\Gamma^2}}.\]
Therefore, by substituting, we find that 
\[A = {\frac{A_0}{\sqrt{(4k/M - \omega_d^2)^2 + \gamma^2\omega_d^2/M}}}\]
As $\gamma$ is very small $$\boxed{A \approx  {\frac{A_0}{4k/M - \omega_d^2}}}$$
\item To decrease the amplitude we have to increase $k$ which is done by reducing length of spring $$A_f = \frac{A_i}{10} \implies 10\left(\frac{k}{M} - \omega_d^2\right)= \frac{k_f}{M} - \omega_d^2 \implies k_f = 10k - 9M\omega_d^2 $$
We know $k \propto \frac{1}{L}$ therefore $$\frac{L_f}{L_i} = \frac{k}{10k - 9M\omega_d^2} \approx \frac{1}{10} \left(1 + \frac{9M\omega_d^2}{10k}\right)$$
\item Like we did in part b, \[A_f = {\frac{A_0}{\sqrt{(4k/M - \omega_d^2)^2 + b^2\omega_d^2/M}}} = \frac{A_i}{10}\] Here $A_i = \frac{A_0}{4K/M - \omega_d^2}$
Therefore $$99\left(\frac{4K}{M} - \omega_d^2\right) = b^2 \frac{\omega_d^2}{M}\implies b = \sqrt{\frac{M}{99\omega_d^2\left(\frac{4K}{M}- \omega_d^2\right)^2}}$$
For $\frac{4K}{M} \gg \omega_d^2$ $$b \approx \sqrt{\frac{M^2}{396K\omega_d^2}\left(1+\frac{M\omega_d^2}{4K}\right)} $$
\end{enumerate}
\end{sol}