\begin{sol}
\begin{enumerate}[label=\textbf{(\alph*)}] 
\item Let $x_1$ be the vertical displacement of the mass $m_1$ and let $x_2$ be the vertical displacement of the mass $m_2$. We then can write the equation of motion as 
\begin{align*}
    m\ddot{x}_1 &= k_C x_1 + k_B (x_1 - x_2) \\
    m\ddot{x}_2 &= k_A x_2 
\end{align*}
We can rewrite this to isolate the equations for both $x_1$ and $x_2$. 
\begin{align*}
    m\ddot{x}_1 &= (k_C + k_B) x_1 - k_B x_2 \\
    m\ddot{x}_2 &= 0 + k_A x_2 
\end{align*}

\item Now, let us write this in matrix format. The $M$ matrix is denoted by 
\[
M = 
\begin{pmatrix}
m & 0 \\
0 & m
\end{pmatrix}.
\]
From our equations of motion, the $K$ matrix has the form 
\[
K = 
\begin{pmatrix}
-k_B - k_C & k_B \\
0 & -k_A
\end{pmatrix}.
\]
Therefore, 
\[M^{-1}K = \begin{pmatrix}
-k_B/m - k_C/m & k_B/m \\
0 & -k_A/m
\end{pmatrix}
\]
This must equal to $\omega^2 I$, or in other words,
\[
\begin{pmatrix}
-k_B/m - k_C/m & k_B/m \\
0 & -k_A/m
\end{pmatrix} = \omega^2\begin{pmatrix}
1 & 0 \\
0 & 1
\end{pmatrix}.
\]
\item The matrix $M^{-1}K - \omega^2 I$ is 
\[M^{-1}K - \omega^2 I = 
\begin{pmatrix}
-k_B/m - k_C/m - \omega^2 & k_B/m \\
0 & -k_A/m - \omega^2
\end{pmatrix}.
\]
To find the eigenvalues of $M^{âˆ’1}K$, we form the determinant 
\begin{align*}
\det [M^{-1}K - \omega^2 I] &= 
\begin{vmatrix}
-k_B/m - k_C/m - \omega^2 & k_B/m \\
0 & -k_A/m - \omega^2
\end{vmatrix} \\
&= (-k_B/m - k_C/m - \omega^2)(-k_A/m - \omega^2) - (k_B/m)(0) \\
&= (-k_B/m - k_C/m - \omega^2)(-k_A/m - \omega^2) = 0.
\end{align*}
Thus, the angular frequencies of the normal modes are 
\[\omega_1^2 = \frac{k_B}{m} + \frac{k_C}{m}, \quad \omega_2^2 = \frac{k_A}{m}.\]
\end{enumerate}
\end{sol}