\begin{sol}
\begin{enumerate}[label=\textbf{(\alph*)}] 
\item Let the distances of each of the masses from their equilibrium points be denoted by $x_1, x_2,$ and $x_3$ in the clockwise direction. We then see that the equations of motions of the masses are defined by 
\begin{align*}
    m\ddot{x}_1 &= -k (x_1 - x_2) - k (x_1 - x_3)\\
    m\ddot{x}_2 &= -k (x_2 - x_1) - k (x_2 - x_3)\\
    m\ddot{x}_3 &= -k (x_3 - x_1) - k (x_3 - x_2)
\end{align*}

\item First, we rewrite our equation of motion to isolate $x_1, x_2$, and $x_3$. By rewriting, we have 
\begin{align*}
    m\ddot{x}_1 &= -2kx_1 + kx_2 + kx_3\\
    m\ddot{x}_2 &= kx_1 - 2kx_2 + kx_3\\
    m\ddot{x}_3 &= kx_1 + kx_2 - 2kx_3
\end{align*}
Using the definition of a normal mode 
\[
\begin{pmatrix}
x_1 \\
x_2 \\
x_3
\end{pmatrix}
= 
\Re \left[
\begin{pmatrix}
A_1 \\
A_2 \\
A_3
\end{pmatrix}
e^{i (\omega t + \phi)}
\right]
\]
we can then rearrange to find 
$$\begin{aligned}- m\omega^{2}A_1 &= -2kA_1 + kA_2 + kA_3 & & 0=\left(-2k + 2m \omega^{2}\right) A_{1}+k A_{2}+k A_{3} \\
-m\omega^{2}A_2 &= kA_1 - 2kA_2 + kA_3 & \Rightarrow \quad & 0= -kA_1 + (-2k + m\omega^2)A_2 + kA_3 \\
-m\omega^2 A_3 &= kA_1 + kA_2 - 2kA_3 & & 0 = kA_1 + kA_2 + (-2k + m\omega^2)A_3
\end{aligned}$$
Now, rewrite in matrix format 
\[
\begin{pmatrix}
-2k + 2m \omega^{2} & k & k \\
-k & -2k + m\omega^2 & k \\
k & k & -2k + m\omega^2
\end{pmatrix}
\begin{pmatrix}
A_1 \\
A_2 \\
A_3
\end{pmatrix}
= 0
\]
To get a solution we need to solve the equation where the determinant of the left matrix is zero.
\[
\begin{vmatrix}
-2k + 2m \omega^{2} & k & k \\
k & -2k + m\omega^2 & k \\
k & k & -2k + m\omega^2
\end{vmatrix}
= 0
\]
If we define $\omega_0^2 = \frac{k}{m}$, then after dividing the matrix by $m$, we yield the equation 
\[
\begin{vmatrix}
-2\omega_0^2 + 2\omega^{2} & \omega_0^2 & \omega_0^2 \\
\omega_0^2 & -2\omega_0^2 + \omega^2 & \omega_0^2 \\
\omega_0^2 & \omega_0^2 & -2\omega_0^2 + \omega^2
\end{vmatrix}
= 0.
\]
After evaluating the determinant we result in the equation 
\[(-2\omega_0^2 + 2\omega^4)[(-2\omega_0^2 + \omega^2)^2 - \omega_0^4] = 0.\]
We now gain two roots of $\omega^2 = 0$ and $\omega^2 = 3\omega_0^2$.

\item We see that in the $\omega^2 = 0$ root, the normal mode is defined by 
\[
\begin{pmatrix}
x_1 \\
x_2 \\ 
x_3
\end{pmatrix}
= 
\begin{pmatrix}
1 \\
1 \\
1
\end{pmatrix}
(At + B)
\]
and corresponds to the masses sliding around the circle at a constant speed. Therefore, there are not really any oscillations exhibited in this mode. 
\end{enumerate}
\end{sol}