\begin{sol}
\begin{enumerate}[label=\textbf{(\alph*)}] 
\item Let us first find the equations of motion without the driving force and then add it in when we are done. Let us denote the upper mass by $m_1$ and the lower mass by $m_2$. We then see that the forces produced by the springs are $ky_1 (t)$ and $ky (2)$. The forces in the spring are then $ky_1 (t)$ and $k (y_2 (t) - y_1 (t))$ respectively. The gravitational force only creates a shift in the equilibrium position but this doesn't affect our equation of motion. This then tells us that our coupled differential equations are:
\begin{align*}
    m_1 \ddot{y}_1 &= + k(y_2(t) - y_1 (t)) - ky_1 (t) + F_0 \cos (\omega_d t) \\ 
    m_2 \ddot{y}_2 &= -k (y_2 (t) - y_1 (t))
\end{align*}
Defining $m_1 = m_2 = m$ and $\omega_0^2 \equiv k/m$, we have 
\begin{align*}
    \ddot{y}_1 &= + \omega_0^2(y_2(t) - 2y_1 (t)) + \frac{F_0}{m}\cos (\omega_d t) \\ 
    \ddot{y}_2 &= -\omega_0^2(y_2 (t) - y_1 (t))
\end{align*}

\item We define 
\[M = \begin{pmatrix}
m & 0 \\ 
0 & m 
\end{pmatrix}, 
\quad 
K = \begin{pmatrix}
+2k & -k \\
-k & +k
\end{pmatrix}
, \quad 
Y = \begin{pmatrix}
y_1 \\ 
y_2
\end{pmatrix}
.\]
With a driving force, our matrix equation is given by 
\[M\ddot{Y} = -K Y + F\cos (\omega_d t).\]

Let us try to consider solutions for $\omega$ without a driving force. Using the definition of a normal mode 
\[
\begin{pmatrix}
x_1 \\
x_2 \\
\end{pmatrix}
= 
\Re \left[
\begin{pmatrix}
A_1 \\
A_2 \\
\end{pmatrix}
e^{i (\omega t + \phi)}
\right]
\]
we can get the equation down to 
$$\begin{aligned}- \omega^{2}A_1 &= -2A_1\omega_0^2 + A_2\omega_0^2 & & 0=\left(-2\omega_0^2 + \omega^{2}\right) A_{1}+ \omega_0^2 A_2 \\
-\omega^{2}A_2 &= A_1\omega_0^2 - A_2 \omega_0^2 & \Rightarrow \quad & 0= \omega_0^2 A_1 + (\omega^2 - \omega_0^2 )A_2 
\end{aligned}$$
Normalizing this into a matrix equation tell us 
\[
\begin{pmatrix}
-2\omega_0^2 + \omega^2 & \omega_0^2 \\
\omega_0^2 & -\omega_0^2 + \omega^2
\end{pmatrix}
\begin{pmatrix}
A_1 \\
A_2
\end{pmatrix}
= 0.\]
To get a solution we need to solve the equation where the determinant of the left matrix is zero
\[
\begin{vmatrix}
-2\omega_0^2 + \omega^2 & \omega_0^2 \\
\omega_0^2 & -\omega_0^2 + \omega^2
\end{vmatrix}
= 0.
\]
Reducing this, we get 
\[(-\omega_0^2 + \omega^2)(-2\omega_0^2 + \omega^2) - \omega_0^4 = -.\]
Simplifying gives us 
\begin{align*}
    2\omega_0^4 - 2\omega^2\omega_0^2 - \omega_0^2 \omega^2 + \omega^4 - \omega_0^4 &= 0 \\
    \omega_0^4 - 3\omega^2\omega_0^2 + \omega^4 &= 0
\end{align*}
This now implies that the roots of this equation are now 
\[\omega_{+} = \sqrt{\frac{(3 + \sqrt{5})k}{2m}}, \quad \omega_{-} = \sqrt{\frac{(3 - \sqrt{5})k}{2m}}.\]
Using these solutions and the fact that 
\[\det (M^{-1}K - \omega^2 I) = (\omega^2 - \omega_{+}^2)(\omega^2 - \omega_{-}^2) = 0\]
to further simplify this problem. Note now that 
\[M^{-1}K = \begin{pmatrix}
2\omega_0^2 & -\omega_0^2 \\ 
-\omega_0^2 & \omega_0^2
\end{pmatrix}
,\quad 
M^{-1}F = \begin{pmatrix}
F_0/m \\
0
\end{pmatrix}
.\]
Using 
\[(M^{-1}K - \omega^2 I)B = M^{-1}F\]
to then expand into matrix form gives us 
\[\begin{pmatrix}
2\omega_0^2 - \omega_d^2 & -\omega_0^2 \\ 
-\omega_0^2 & \omega_0^2 - \omega_d^2
\end{pmatrix}
\begin{pmatrix}
B_1 \\
B_2
\end{pmatrix}
= 
\begin{pmatrix}
F_0/m \\
0
\end{pmatrix}
\]
We can go ahead and solve it directly to get $B_1$ and $B_2$ or we can use “Cramer’s Rule” which is a useful rule when solving a large number of coupled oscillators. First define:
\[E^{\leftrightarrow} = \begin{pmatrix}
2\omega_0^2 - \omega_d^2 & -\omega_0^2 \\ 
-\omega_0^2 & \omega_0^2 - \omega_d^2
\end{pmatrix},
\quad 
D^{\rightarrow} = \begin{pmatrix}
F_0 /m \\
0
\end{pmatrix}
.\]
To use Cramer’s rule, use one column from $E^{\leftrightarrow}$ and $D^{\rightarrow}$
\begin{align*}
    B_1 &= \frac{|(D^{\rightarrow})()|}{\det E^{\leftrightarrow}} \\
    &= \frac{\begin{pmatrix}
    F_0/m & -\omega_0^2 \\
    0 & \omega_0^2 - \omega_d^2
    \end{pmatrix}}{(\omega^2 - \omega_{+}^2)(\omega^2 - \omega_{-}^2)} \\
    &= \frac{\frac{F_0}{m} (\omega_0^2 - \omega_d^2)}{(\omega^2 - \omega_{+}^2)(\omega^2 - \omega_{-}^2)}
\end{align*}
Which explodes when $\omega_d = \omega_{+}, \omega_{-}$ which are the frequencies of the normal modes. Similarly:
\begin{align*}
    B_2 &= \frac{|()(D^{\rightarrow})|}{\det E^{\leftrightarrow}} \\
    &= \frac{\begin{pmatrix}
    2\omega_0^2 & F_0/m \\
    -\omega_0^2 & 0
    \end{pmatrix}}{(\omega^2 - \omega_{+}^2)(\omega^2 - \omega_{-}^2)} \\
    &= \frac{\frac{F_0}{m}\left(\frac{\omega_0^2}{m}\right)}{(\omega^2 - \omega_{+}^2)(\omega^2 - \omega_{-}^2)} \\
\end{align*}
The full solution is given by 
\begin{align*}
    y_1 &= \alpha \cos (\omega_{+}t + \phi) + \beta \cos (\omega_{-}t + \phi) + B_1 \cos (\omega_d t)
\end{align*}
\end{enumerate}
\end{sol}