\begin{sol}
We can solve this generally, but before we do so, we need to state and prove the following lemmas:
\newline
\begin{lemma}
If $\displaystyle A=\binom{u_1}{u_2}$ is a $1\times 2$ matrix then $A^\dagger A = |u_1|^2+|u_2|^2$
\end{lemma}

\begin{prooof}
By definition, the Hermitian $A^\dagger$ can be written as $\begin{pmatrix}u_1^* & u_2^*\end{pmatrix}$ so their product gives:
$$\begin{pmatrix}u_1^* & u_2^*\end{pmatrix}
\begin{pmatrix}u_1 \\ u_2\end{pmatrix} = u_1^*u_1 + u_2^*u_2 = |u_1|^2+|u_2|^2
$$
\end{prooof}
Thus, when the question acts for the conservation of probability, an equivalent statement is to set the equality
$$u^\dagger u=u'^\dagger u' = 1$$
\begin{lemma}
If $R$ is a $2\times 2$ matrix and $u$ is a $1\times2$ matrix, then $(Ru)^\dagger=u^\dagger R^\dagger$
\end{lemma}
\begin{prooof}
Generalize our matrices as $\displaystyle R = \begin{pmatrix} a & b \\ c & d\end{pmatrix}$ and $\displaystyle u=\binom{u_1}{u_2}$. Then:
\begin{align*}
    (Ru)^\dagger &= \left[\begin{pmatrix} a & b \\ c & d\end{pmatrix}\binom{u_1}{u_2}\right]^\dagger \\
    &= \begin{pmatrix}au_1+bu_2 \\ cu_1+du_2\end{pmatrix}^\dagger \\
    &= \begin{pmatrix}a^*u_1^*+b^*u_2^* & c^*u_1^*+d^*u_2^*\end{pmatrix}
\end{align*}
and similarly
\begin{align*}
    u^\dagger R^\dagger &= \begin{pmatrix}u_1^* & u_2^*\end{pmatrix}\begin{pmatrix} a^* & c^* \\ b^* & d^*\end{pmatrix} \\
    &= \begin{pmatrix}a^*u_1^*+b^*u_2^* & c^*u_1^*+d^*u_2^*\end{pmatrix}
\end{align*}
\end{prooof}
With these out of the way, the proof becomes trivial. All we need to show is that:
\begin{align*}
    u'^\dagger u' &= (Ru)^\dagger (Ru) \\
    &= u^\dagger (R^\dagger R) u
\end{align*}
If we wish to end up with the equality:
$$u^\dagger u=u'^\dagger u' = 1$$
then it must be true that $R^\dagger R=I$, or in other words: $R$ is unitary.
\end{sol}