\begin{sol}
\begin{enumerate}[label=\textbf{(\alph*)}]
\item Let us first write the phase in terms of the momentum and energy of the wave:
$$\frac{1}{\hbar}\phi=\hbar kx-\hbar \omega t = px - \frac{p^2}{2m}t$$
Where momentum undergoes the transformation
$$p'=p-mv$$
Thus, this must be equal to:
\begin{align*}
    \frac{1}{\hbar}\phi &= (p'+mv)(x'+vt)-\frac{(p'+mv)^2}{2m}t \\
    &= p'x + \cancel{p'vt}+mvx'+mv^2t-\frac{p'^2}{2m}t-\cancel{p'vt}-\frac{1}{2}mv^2t \\
    &= p'x + mv(x-vt) - \frac{p'^2}{2m}t+\frac{1}{2}mv^2t \\
    &= p'x+mvx-mv^2t - E't + \frac{1}{2}mv^2t \\
    &= p'x-E't+mvx-\frac{1}{2}mv^2t
\end{align*}
The first two terms are the phase of the primed wavefunction. The last two terms gives rise to $f(x,t)$ to be:
$$f(x,t)=\exp\left(\frac{i}{\hbar}\left(mvx-\frac{1}{2}mv^2t\right)\right)$$
\end{enumerate}
\end{sol}